ref as array

ulib/experimental/Steel.C.Model.Array.fst
@@ -760,3 +760,150 @@ let join
   A.change_equal_slprop (pts_to a _) (pts_to a _)
 
 #pop-options
+
+#restart-solver
+let array_as_one_ref_iso
+  (#t: Type)
+  (p: pcm t)
+: Tot (isomorphism (array_pcm p 1sz) p)
+= assert_norm (size_v 1sz == 1);
+  let c = cell p 1sz 0sz in
+  let c1 = c.conn_large_to_small in
+  let c2 = c.conn_small_to_large in
+  Steel.C.Model.Connection.mkisomorphism
+    c1
+    c2
+    ()
+    (Steel.C.Model.Connection.is_inverse_of_intro
+      c2.Steel.C.Model.Connection.morph
+      c1.Steel.C.Model.Connection.morph
+      (fun x ->
+        array_pcm_carrier_ext t 1sz (c2.Steel.C.Model.Connection.morph (c1.Steel.C.Model.Connection.morph x)) x (fun i ->
+          ()
+        )
+      )
+    )
+    (fun x -> ())
+    (fun x -> ())
+
+#restart-solver
+let array_as_one_ref_iso_eq
+  (#t: Type)
+  (p: pcm t)
+: Lemma
+  (
+    let _ = assert_norm (size_v 0sz == 0) in
+    let _ = assert_norm (size_v 1sz == 1) in
+    let _ : squash (size_v 0sz < size_v 1sz) = () in
+    connection_of_isomorphism (array_as_one_ref_iso p) == cell p 1sz 0sz
+  )
+= assert_norm (size_v 0sz == 0);
+  assert_norm (size_v 1sz == 1);
+  let l = (connection_of_isomorphism (array_as_one_ref_iso p)) in
+  let m = (cell p 1sz 0sz) in
+  connection_eq_gen
+    l
+    m
+    ()
+    (fun x y f v ->
+      connection_of_isomorphism_fpu_eq (array_as_one_ref_iso p) x y f v;
+      assert_norm ((m.conn_lift_frame_preserving_upd ({ fpu_lift_dom_x = x; fpu_lift_dom_y = y; fpu_lift_dom_f = f; })).fpu_f v == struct_field_lift_fpu' (array_elements_pcm p 1sz) 0sz x y f v);
+      assert (connection_of_isomorphism_fpu' (array_as_one_ref_iso p) x y f v `feq` struct_field_lift_fpu' (array_elements_pcm p 1sz) 0sz x y f v);
+      assert ((l.conn_lift_frame_preserving_upd ({ fpu_lift_dom_x = x; fpu_lift_dom_y = y; fpu_lift_dom_f = f; })).fpu_f v == (m.conn_lift_frame_preserving_upd ({ fpu_lift_dom_x = x; fpu_lift_dom_y = y; fpu_lift_dom_f = f; })).fpu_f v)
+    )
+
+let array_of_ref_conn
+  (#t: Type)
+  (p: pcm t) 
+: Tot (connection p (array_pcm p 1sz))
+= connection_of_isomorphism (isomorphism_inverse (array_as_one_ref_iso p))
+
+let g_array_of_ref
+  (#t: Type)
+  (#p: pcm t)
+  (r: ref p)
+: Ghost (array p)
+    (requires True)
+    (ensures (fun a ->
+      size_v a.base_len == 1 /\
+      size_v a.len == 1
+    ))
+= assert_norm (size_v 1sz == 1);
+  {
+    base_len = _;
+    base = ref_focus r (array_of_ref_conn p);
+    offset = 0sz;
+    len = 1sz;
+    prf = ();
+  }
+
+let ref_of_array_of_ref_base
+  (#t: Type)
+  (#p: pcm t)
+  (r: ref p)
+: Lemma
+  (ref_of_array (g_array_of_ref r) == ref_focus r (array_of_ref_conn p))
+= ref_of_array_id (g_array_of_ref r)
+
+#push-options "--split_queries"
+
+#restart-solver
+let ref_of_array_of_ref
+  (#t: Type)
+  (#p: pcm t)
+  (r: ref p)
+: Lemma
+  (ref_focus (ref_of_array (g_array_of_ref r)) (cell p 1sz 0sz) == r)
+= ref_of_array_of_ref_base r;
+  ref_focus_comp r (array_of_ref_conn p) (cell p 1sz 0sz); 
+  array_as_one_ref_iso_eq p;
+  connection_of_isomorphism_inverse_left (array_as_one_ref_iso p);
+  ref_focus_id r
+
+#pop-options
+
+#restart-solver
+let ghost_array_of_ref
+  (#opened: _)
+  (#t: Type)
+  (#p: pcm t)
+  (#v: t)
+  (r: ref p)
+: A.SteelGhostT unit opened
+    (R.pts_to r v)
+    (fun _ -> pts_to (g_array_of_ref r) (Seq.create 1 v))
+= assert_norm (size_v 0sz == 0);
+  assert_norm (size_v 1sz == 1);
+  let v' : array_pcm_carrier t 1sz = field_to_struct_f (array_elements_pcm p 1sz) 0sz v in
+  assert (seq_of_array_pcm_carrier v' `Seq.equal` Seq.create 1 v);
+  R.gfocus r (array_of_ref_conn p) _ v';
+  ref_of_array_of_ref_base r; 
+  intro_pts_to1 _ _ _ _
+
+#restart-solver
+let array_of_ref
+  (#t: Type)
+  (#p: pcm t)
+  (#v: Ghost.erased t)
+  (r: ref p)
+: Steel (array p)
+    (R.pts_to r v)
+    (fun a -> pts_to a (Seq.create 1 (Ghost.reveal v)))
+    (fun _ -> True)
+    (fun _ a _ -> a == g_array_of_ref r)
+= assert_norm (size_v 0sz == 0);
+  assert_norm (size_v 1sz == 1);
+  let v' : Ghost.erased (array_pcm_carrier t 1sz) = Ghost.hide (field_to_struct_f (array_elements_pcm p 1sz) 0sz v) in
+  assert (seq_of_array_pcm_carrier v' `Seq.equal` Seq.create 1 (Ghost.reveal v));
+  let r' = R.focus r (array_of_ref_conn p) _ v' in
+  let a : array p = {
+    base_len = 1sz;
+    base = r';
+    offset = 0sz;
+    len = 1sz;
+    prf = ();    
+  }
+  in
+  ref_of_array_of_ref_base r;
+  intro_pts_to1 a _ _ _;
+  A.return a
